\documentclass[12pt]{article}
 
\usepackage[margin=1in]{geometry} 
\usepackage{amsmath,amsthm,amssymb,scrextend}
\usepackage{fancyhdr}
\pagestyle{fancy}
 
\newcommand{\N}{\mathbb{N}}
\newcommand{\Z}{\mathbb{Z}}
\newcommand{\I}{\mathbb{I}}
\newcommand{\R}{\mathbb{R}}
\newcommand{\Q}{\mathbb{Q}}
\renewcommand{\qed}{\hfill$\blacksquare$}
\let\newproof\proof
% \renewenvironment{proof}{\begin{addmargin}[1em]{0em}\begin{newproof}}{\end{newproof}\end{addmargin}\qed}
 
\newenvironment{theorem}[2][Theorem]{\begin{trivlist}
\item[\hskip \labelsep {\bfseries #1}\hskip \labelsep {\bfseries #2.}]}{\end{trivlist}}
\newenvironment{lemma}[2][Lemma]{\begin{trivlist}
\item[\hskip \labelsep {\bfseries #1}\hskip \labelsep {\bfseries #2.}]}{\end{trivlist}}
\newenvironment{problem}[2][Problem]{\begin{trivlist}
\item[\hskip \labelsep {\bfseries #1}\hskip \labelsep {\bfseries #2.}]}{\end{trivlist}}
\newenvironment{exercise}[2][Exercise]{\begin{trivlist}
\item[\hskip \labelsep {\bfseries #1}\hskip \labelsep {\bfseries #2.}]}{\end{trivlist}}
\newenvironment{reflection}[2][Reflection]{\begin{trivlist}
\item[\hskip \labelsep {\bfseries #1}\hskip \labelsep {\bfseries #2.}]}{\end{trivlist}}
\newenvironment{proposition}[2][Proposition]{\begin{trivlist}
\item[\hskip \labelsep {\bfseries #1}\hskip \labelsep {\bfseries #2.}]}{\end{trivlist}}
\newenvironment{corollary}[2][Corollary]{\begin{trivlist}
\item[\hskip \labelsep {\bfseries #1}\hskip \labelsep {\bfseries #2.}]}{\end{trivlist}}
 
\begin{document}
 
% --------------------------------------------------------------
%                         Start here
% --------------------------------------------------------------

\title{Assignment 1 \\ CPSC 331} % Title and subtitle
\author{Guransh Mangat, 30061719 \\ Daniel Contreras, 10080311 \\ Steven Ferguson, 30037518\\ \\ \\ \\ \\ \\ \\ \\ \\ \\ \\ \\ 
\\ \\ \\ \\ \\ \\ \\ \\ \\ \\ \\ \\ \\ \\ \\ \\  }
\date{}


\lhead{CPSC 331}
\chead{Assignment 1}
\rhead{September 2019}
 
\maketitle{}

% --------------------------------------------------------------
%                         1
% --------------------------------------------------------------

\begin{problem}{1}
    Suppose that the function $f(n)=n$ is a bound function.
\end{problem}

\begin{proof}
    Since $n$ is an integer input, this is an \textit{integer-valued} function.\\ \\ When the 
    recursive function is applied in \textit{line 9}, the value of n is reduced by at least 1 
    ($(n-1), (n-3) \ and \ (n-4)$). \newline \newline $n$ is a non negative integer, which means 
    $n \geq 0$. Thus it is only possible that $ f(n) = n \leq 0$ when n = 0. In that case, the test 
    at \textit{line 1} passes, the execution continues at \textit{line 1} and the execution ends 
    without having to call the recursive function repeatedly. \newline \newline Hence, the function 
    $f(n) = n$ is a bound function. 
\end{proof}

% --------------------------------------------------------------
%                         2
% --------------------------------------------------------------

\begin{problem}{2}
    Prove that the smacG algorithm correctly solves the "MacGonagall Mystery Computation" problem.
\end{problem}

\begin{proof}
    \noindent This theorem will be proved by induction on $n$. The strong form of mathematical induction will be used, and base cases of $n = 0, 1, 2 ,3$ will each be considered in the basis.\\
    
    \noindent Basis: Suppose, first $n = 0$: \newline During the execution of algorithm smacG on input $n$, the test at line 1 succeeds and the execution continues at line 2. This causes the execution to terminate with the value of $M_0 = 1$ returned at output - as required for this case \\ 
    
    \noindent Suppose, next, $n = 1$: \\ During the execution of the algorithm smacG, the test at line 1 fails and the execution continues with test at line 3. \\ This test succeeds, so the execution continues at line 4. This causes the execution of algorithm to terminate with value of $M_1 = 0$ returned as output- as required by this case \\ 
    
    \noindent Suppose, $n = 2$: \\ During the execution of the algorithm smacG, the test at line 1 and line 3 fails, and the execution continues with test at line 5. \\ This test succeeds, so the execution continues with line 6. This causes the execution of the algorithm to terminate with the value of $M_2 = 5$ returned as output - as require by this case. \\ 
    
    \noindent Suppose, n = 3: \\ During the execution of the algorithm smacG, the test at line 1, line 3 and line 5 fails, and the execution continues with the test at line 7. \\ This test succeeds, so the execution continues with line 8. This causes the execution of the algorithm to terminate with the value of $M_3 = 8$ returned as output - as required by this case. \\ 
    
    \noindent \textit{Inductive Step: } Let $k$ be an integer such that $k \geq 3$. \\
    
    \noindent \textbf{Inductive Hypothesis: } Suppose $n$ is a non-negative integer such that $ 0 \leq n \leq k$. If the algorithm smacG is executed given n as input then this execution of the algorithm eventually terminates, with the $n^{th}$ MacGonagall number, $M_n$ returned as output. \\
    
    \noindent \textbf{Inductive Claim: } If the algorithm smacG is executed given $n = k + 1$ as input then this execution of the algorithm eventually terminates, with the $k+1^{st}$ MacGonagall number $M_{k+1} = M_n$ returned as output. \\
    
    \noindent Suppose the algorithm smacG is executed with $n= k + 1$ given as input. Since $k$ is an integer such that $k \geq 3$, $n$ is an integer such that $n \geq 4$.
    
    \noindent Since $n \geq 4$, the test at line 1, line 3, line 5 and line 7 fails and the algorithm continues at line 8. 
    
    \noindent Line 9 includes a recursive execution of this algorithm with the input $2 \times (n-1)$. Since $n = k + 1 \geq 4, 0 \leq n-1 = k \leq k$, and it follows by the \textbf{inductive hypothesis} that this recursive execution of the algorithm eventually ends with $M_{n-1} = M_k$ returned as output
    
    \noindent Line 9 also includes a recursive execution of this algorithm with the input $-2 \times (n-3)$. Since $n = k+1 \geq 4, 0 \leq n-3 = k-2 \leq k$, and it follows the \textbf{inductive hypothesis} that this recursive execution of the algorithm eventually ends with $M_{n-3} = M_{k-2}$ returned as output.
    
    \noindent Line 9 also includes a recursive execution of algorithm with the input $n-4$. Since $n = k+1 \geq 4, 0 \leq n-4 = k-3 \leq 4$, and it follows by the \textbf{inductive hypothesis} that this recursive function of the algorithm eventually ends with $M_{n-4} = M_{k-3}$ returned as output.
    
    \noindent Once the execution of algorithm ends, since, $k+1 \geq 4$, it follows the definition of $M_{k+1}$, that the value returned as output is: \\ \\
    $2 \times M_{n-1} - 2 \times M_{n-3} + M_{n-4} = 2 \times M_{k} -2 \times M_{k-2} + M_{k-3} = M_{k+1}$ \\ 
    
    \noindent as required to establish the \textbf{inductive claim.} \\ \\
    This results now follows by induction on n.
\end{proof}


% --------------------------------------------------------------
%                         3
% --------------------------------------------------------------

\begin{problem}{3}
\end{problem}

\begin{proof}
\end{proof}


% --------------------------------------------------------------
%                         4
% --------------------------------------------------------------

\begin{problem}{4}
\end{problem}

\begin{proof}
    In order to determine the number of steps included in the execution of $T_{smacG}(n)$, we will define the running time of each step in the algorithm to be \textit{one}.\\

    \noindent Using the uniform cost criterion to define $T_{smacG}(n)$: \\
    
    \noindent The algorithm executes 2 steps (at lines 1 and 2) if it is executed when $n = 0$. \\
    \noindent The algorithm executes 3 steps (at lines 1, 3, 4) if it is executed when $n = 1$. \\
    \noindent The algorithm executes 4 steps (at lines 1, 3, 5, 6) if it is executed when $n = 2$. \\
    \noindent The algorithm executes 5 steps (at lines 1, 3, 5, 7, 8) if it is executed when $n = 3$. \\
    
    
    \[ \hspace*{-17mm}T_{smacG}(n) = 
        \begin{cases} 
          2 & if n = 0, \\
          3 & if n = 1, \\
          4 & if n = 2, \\
          5 & if n = 3, \\
          T_{smacG}(n-1) + T_{smacG}(n-3) + T_{smacG}(n-4) + 5 & if n \geq 4.
       \end{cases}
    \]
    
    \noindent We can use this recurrence to show the following:\\
    
    \begin{flalign*}
        \hspace*{5mm}T_{smacG}(0) &= 2 &&\text{(by definition of $T_{smacG}(n)$)} \\ \\
        \hspace*{5mm}T_{smacG}(1) &= 3 &&\text{(by definition of $T_{smacG}(n)$)} \\ \\
        \hspace*{5mm}T_{smacG}(2) &= 4 &&\text{(by definition of $T_{smacG}(n)$)} \\ \\
        \hspace*{5mm}T_{smacG}(3) &= 5 &&\text{(by definition of $T_{smacG}(n)$)} \\ \\
        \hspace*{5mm}T_{smacG}(4) &= T_{smacG}(4-1) + T_{smacG}(4-3) + T_{smacG}(4-4) + 5  &&\text{} \\
        &= T_{smacG}(3) + T_{smacG}(1) + T_{smacG}(0) + 5  &&\text{} \\
        &= 5 + 3 + 2 + 5  &&\text{} \\
        &= 15. \\ \\
        \hspace*{5mm}T_{smacG}(5) &= T_{smacG}(5-1) + T_{smacG}(5-3) + T_{smacG}(5-4) + 5 &&\text{} \\
        &= T_{smacG}(4) + T_{smacG}(2) + T_{smacG}(1) + 5 &&\text{} \\
        &= 15 + 4 + 3 + 5 &&\text{} \\
        &= 27.
    \end{flalign*}

\end{proof}


% --------------------------------------------------------------
%                         5
% --------------------------------------------------------------

\begin{problem}{5} 
    Suppose that $T_{smacG}$ is a function of the non-negative integers such that, for every integer 
    $n \geq 0$,

    \[  
        \hspace*{-22mm}T_{smacG}(n) =
        \begin{cases} 
        2 & n = 0 \\
        3 & n = 1 \\
        4 & n = 2 \\
        5 & n = 3 \\
        T_{smacG}(n-1) + T_{smacG}(n-3) + T_{smacG}(n-4) + 5 & n \geq 4 
        \end{cases}
    \]

    \noindent then $T_{smacG}(n) \geq \left(\frac{3}{2}\right)^n$ for every non-negative integer $n$ and therefore
    the number of steps executed by the $smacG$ algorithm is at least exponential in its input.
\end{problem}

\begin{proof} 
This will be established by induction on $n$. The strong form of mathematical induction will be used 
and the cases $n = 0$, $n=1$, $n=2$ and $n=3$ will be considered in the basis.\\

\noindent \textit{Basis}. If $n=0$, then $T_{smacG}\left(n\right) = T_{smacG}\left(0\right) = 2$, and 
\begin{flalign*}
    \hspace*{5mm}T_{smacG}(n) &\geq \left(\frac{3}{2}\right)^n &&\text{} \\
    T_{smacG}\left(0\right) &\geq \left(\frac{3}{2}\right)^0 &&\text{} \\
    2 &\geq 1 &&\text{} \\
\end{flalign*}
as required. If $n=1$, then $T_{smacG}\left(n\right) = T_{smacG}\left(1\right) = 3$, and 
\begin{flalign*}
    \hspace*{5mm}T_{smacG}\left(n\right) &\geq \left(\frac{3}{2}\right)^n &&\text{} \\
    T_{smacG}\left(1\right) &\geq \left(\frac{3}{2}\right)^1 &&\text{} \\
    3 &\geq \frac{3}{2} &&\text{} \\
\end{flalign*}
as required. If $n=2$, then $T_{smacG}\left(n\right) = T_{smacG}\left(2\right) = 4$, and 
\begin{flalign*}
    \hspace*{5mm}T_{smacG}\left(n\right) &\geq \left(\frac{3}{2}\right)^n &&\text{} \\
    T_{smacG}\left(2\right) &\geq \left(\frac{3}{2}\right)^2 &&\text{} \\
    4 &\geq \frac{9}{4} &&\text{} \\
\end{flalign*}
as required. If $n=3$, then $T_{smacG}\left(n\right) = T_{smacG}\left(3\right) = 5$, and 
\begin{flalign*}
    \hspace*{5mm}T_{smacG}\left(n\right) &\geq \left(\frac{3}{2}\right)^n &&\text{} \\
    T_{smacG}\left(3\right) &\geq \left(\frac{3}{2}\right)^3 &&\text{} \\
    5 &\geq \frac{27}{8} &&\text{} \\
\end{flalign*}
as required. \\

\noindent \textit{Inductive Step}. Let $k \geq 4$ be an integer. It is necessary and sufficient
to use the following \\

\underline{Inductive Hypothesis}: $T_{smacG}\left(m\right) \geq \left(\frac{3}{2}\right)^{m}$
for every integer $m$ such that $0 \leq m \leq k$. \\

\noindent to prove the following \\

\underline{Inductive Claim}: $T_{smacG}\left(k+1\right) \geq \left(\frac{3}{2}\right)^{k+1}$ \\

\noindent Now, since $k+1 > 4$,

\begin{flalign*}
    \hspace*{5mm}T_{smacG}(k+1) &= T_{smacG}(k) + T_{smacG}(k-2) + T_{smacG}(k-3) + 5 \\
    &\geq \left(\frac{3}{2}\right)^{k} + \left(\frac{3}{2}\right)^{k-2} + \left(\frac{3}{2}\right)^{k-3} + 5 &&\text{(by inductive hypothesis)} \\
    &= \left(\frac{3}{2}\right)^{k+1} + \left(\left(\frac{3}{2}\right)^{-1} + \left(\frac{3}{2}\right)^{-3} + \left(\frac{3}{2}\right)^{-4}\right) + 5 \\
    &= \left(\frac{3}{2}\right)^{k+1} \left(\frac{94}{81}\right) + 5 \\
    &\geq \left(\frac{3}{2}\right)^{k+1} \left(\frac{94}{81}\right) \\
    &\geq \left(\frac{3}{2}\right)^{k+1} &&\text{(because $\frac{94}{81} > 1$)}\\
\end{flalign*}

\noindent thus establishing the inductive claim, as needed. Therefore, by principle of induction 
$T_{smacG}\left(n\right) \geq \left(\frac{3}{2}\right)^{n}$ for all non-negative integers $n$.

\end{proof} 

% --------------------------------------------------------------
%                         6
% --------------------------------------------------------------

\begin{problem}{6}
\end{problem}

\begin{proof}
\end{proof}


% --------------------------------------------------------------
%                         7
% --------------------------------------------------------------

\begin{problem}{7}
\end{problem}

\begin{proof}
\end{proof}


% --------------------------------------------------------------
%                         8
% --------------------------------------------------------------

\begin{problem}{8}
\end{problem}

\begin{proof}
\end{proof}


% --------------------------------------------------------------
%                         9
% --------------------------------------------------------------

\begin{problem}{9}
\end{problem}

\begin{proof}
\end{proof}


% --------------------------------------------------------------
%                         10
% --------------------------------------------------------------

\begin{problem}{10}
\end{problem}

\begin{proof}
\end{proof}


% --------------------------------------------------------------
%                         11
% --------------------------------------------------------------

\begin{problem}{11}
\end{problem}

\begin{proof}
\end{proof}


% --------------------------------------------------------------
%                         12
% --------------------------------------------------------------

\begin{problem}{12}
\end{problem}

\begin{proof}
\end{proof}


% --------------------------------------------------------------
%                         13
% --------------------------------------------------------------

\begin{problem}{13}
\end{problem}

\begin{proof}
\end{proof}


% --------------------------------------------------------------
%                         14
% --------------------------------------------------------------
    
\begin{problem}{14}
\end{problem}

\begin{proof}
\end{proof}

 
% --------------------------------------------------------------
%     You don't have to mess with anything below this line.
% --------------------------------------------------------------
 
\end{document}
